ex2/lists.v
@@ -5,17 +5,82 @@ Import ListNotations.
 Print list.
 Print rev.
 
+(* Q1. Define is_sorted.  (returns a Prop.)  *)
+Fixpoint is_sorted {A: Type} (l : list A) (R: A -> A -> Prop) : Prop :=
+  match l with
+  | x :: ((y :: _) as xs) => R x y /\ is_sorted xs R
+  | _ => True
+  end.
 
-(* Q1. Define `is_sorted`.  (should return a Prop.)  *)
 
-
-(* Show that this list is sorted. *)
+(* Q2. Show that this list is sorted. *)
 Lemma warm_up : is_sorted [3;5;9] le.
+  simpl.
+  split.
+  - apply le_S, le_S, le_n.
+  - simpl. split. apply le_S, le_S, le_S, le_S, le_n.
+  trivial.
+Qed.
 
 
-(* Q2. Prove that an ascending list of nat, when reversed, 
+(* Q3. Prove that an ascending list of nat, when reversed, 
  *     becomes a descending list. *)
 
-(*     Don't forget to use the _hint_ when proving it. *)
+(* The following are utility definitions to simplify readability *)
+Definition is_asc (l : list nat) := is_sorted l le.
+Definition is_desc (l : list nat) := is_sorted l ge.
 
-Theorem rev_asc_desc : ...
+Lemma aux1 : forall (A : Set) (l : list A) R a b,
+      is_sorted (l ++ [a]) R ->
+      R a b ->
+      is_sorted (l ++ [a;b]) R.
+Proof.
+  intros A l R a b Hsorted Hab.
+  induction l as [| x xs IH].
+  (* Case: l = [] *)
+  - simpl. split; assumption.
+  (* Case: l = x :: xs*)
+  - simpl in *. destruct xs as [| y ys].
+    (* Case: xs = [] -> l = [x]*)
+    + simpl in *. simpl.
+      destruct Hsorted as [Hxa _].
+      split.
+      * exact Hxa.
+      * split.
+        -- exact Hab.
+        -- constructor.
+    (* Case: xs = y :: ys *)
+    + simpl in Hsorted.
+      destruct Hsorted as [Hxy Hrest].
+      simpl.
+      split.
+      * exact Hxy.
+      * apply IH. exact Hrest.
+Qed.
+
+Definition le_ge := fun n m (H: n <= m) => H : m >= n.
+
+Lemma rev_cons : forall (A : Type) (x : A) (xs : list A),
+  rev (x :: xs) = rev xs ++ [x].
+Proof.
+  intros. reflexivity.
+Qed.
+
+
+Theorem rev_asc_desc : forall (l: list nat), is_asc l -> is_desc (rev l).
+Proof.
+  intros l Hasc.
+  induction l as [| x xs IH].
+  - simpl. constructor.
+  - simpl in *. simpl in Hasc.
+    destruct xs as [| y ys].
+    + simpl. constructor.
+    + simpl in Hasc. 
+      destruct Hasc as [Hxy Hsorted].
+      rewrite rev_cons.
+      rewrite <- app_assoc.
+      apply (@aux1 nat (rev ys) ge y x).
+      * apply IH. exact Hsorted.
+      * apply le_ge. exact Hxy.
+Qed.
+
